# Homework Eight

# Prove

将{x1, ^x1 V x2, ^x1 V x3, ^x2 V ^x3}转化为对应的整数表达式,
结果为  
1 - x1 + x1 * (1 - x2) + x1 * (1 - x3) + x2 * x3  
= 1 - x1 * x2 + x1 - x1 * x3 + x2 * x3  
= 1 - x2 - x3  - x1 + x1 *  x2 + x1 * x3  
= 1 + x1 - x1 * (x 2 + x3 ) + x1 * x2 * x3 + x2 * x3 - x1 * x2 * x3  
= 1 + x1 * (1 - x2 ) * (1 - x3) + (1 - x1) * x2 * x3

而{0, x1 V x2 V x3, x1 V ^ x2 ^ x3} 对应的表达式为  
1 + x1 * (1 - x2 ) * (1 - x3) + (1 - x1) * x2 * x3  
所以两者等价

# Find Example
1. {x1, x2, ^x1 V ^x2} 和 {0, x1 V x2}   
第一个: (1 - x1) + (1 - x2) + x1* x2 = 2 - x1 - x2 + x1 * x2  
第二个: 1 + (1 - x1) * (1 - x2) = 1 + 1 - x1 - x2 + x1 * x2 = 2 - x1 - x2 + x1 * x2  
所以等价

2. {^x1 V ^ x3, ^x1 V x3 ,  x1 V x2, ^x2} 和 {0, ^x1 V ^x2}  
第一个:  
x1 * x3 + x1 * (1- x3) + (1 - x1) * (1 - x2) + x2  
= x1 + x2 + 1 - x1 - x2 + x1 * x2  
= 1 + x1 * x2  
第二个:  
1 + x1 * x2  
所以等价 